prove sval_refine_get

core/AssertionLang.v
@@ -4,8 +4,7 @@ Require Import Poulet4.Syntax.
 Require Import Poulet4.Semantics.
 Require Import Poulet4.Value.
 Require Import ProD3.core.Coqlib.
-(* Only depends on Hoare for sval_refine. *)
-Require Import ProD3.core.Hoare.
+Require Import ProD3.core.SvalRefine.
 Require Import Coq.Numbers.BinNums.
 Open Scope type_scope.
 
@@ -131,65 +130,6 @@ Definition gen_sval (typ: P4Type) (upds: list (path * Sval)): option Sval :=
   | None =>
       None
   end.
-
-(* Another version of get and update. *)
-
-Definition has_field (f : ident) (sv : Sval) : bool :=
-  match sv with
-  | ValBaseStruct fields =>
-      is_some (AList.get fields f)
-  | ValBaseHeader fields (Some true) =>
-      is_some (AList.get fields f)
-  | _ => false
-  end.
-
-Definition get (f : ident) (sv : Sval) : Sval :=
-  match sv with
-  | ValBaseStruct fields =>
-      force ValBaseNull (AList.get fields f)
-  | ValBaseHeader fields _ =>
-      force ValBaseNull (AList.get fields f)
-  | _ => ValBaseNull
-  end.
-
-Definition update (f : ident) (f_sv : Sval) (sv : Sval) : Sval :=
-  match sv with
-  | ValBaseStruct fields =>
-      ValBaseStruct (force fields (AList.set fields f f_sv))
-  | ValBaseHeader fields (Some true) =>
-      ValBaseHeader (force fields (AList.set fields f f_sv)) (Some true)
-  | _ => sv
-  end.
-
-Lemma get_some_get_set : forall {A} (l : AList.StringAList A) k (l' : AList.StringAList A) v1 v2,
-  AList.get l k = Some v1 ->
-  AList.get (force l' (AList.set l k v2)) k = Some v2.
-Proof.
-  intros.
-  erewrite AList.get_some_set by eauto.
-  apply AList.set_some_get.
-Qed.
-
-Lemma get_update : forall sv f f_sv,
-  has_field f sv ->
-  get f (update f f_sv sv) = f_sv.
-Proof.
-  intros.
-  destruct sv; try solve [inv H0].
-  - unfold get, update, has_field in *.
-    destruct (AList.get fields f) eqn:?.
-    + erewrite get_some_get_set by eauto.
-      auto.
-    + inv H0.
-  - destruct is_valid as [[] | ].
-    * unfold get, update, has_field in *.
-      destruct (AList.get fields f) eqn:?.
-      + erewrite get_some_get_set by eauto.
-        auto.
-      + inv H0.
-    * inv H0.
-    * inv H0.
-Qed.
 
 (* Definition extract (v : Val) (f : ident) : option Val :=
   match v with
