core/Members.v
@@ -1,0 +1,81 @@
+Require Import Coq.Strings.String.
+Require Import Poulet4.Typed.
+Require Import Poulet4.Syntax.
+Require Import Poulet4.Semantics.
+Require Import Poulet4.Value.
+Require Import ProD3.core.Coqlib.
+Require Import Coq.Numbers.BinNums.
+Open Scope type_scope.
+
+Section Members.
+
+Context {tags_t: Type} {tags_t_inhabitant : Inhabitant tags_t}.
+Notation Val := (@ValueBase bool).
+Notation Sval := (@ValueBase (option bool)).
+Notation Lval := ValueLvalue.
+
+Notation ident := (string).
+Notation path := (list ident).
+Notation P4Int := (P4Int.t tags_t).
+Notation P4String := (P4String.t tags_t).
+Notation P4Type := (@P4Type tags_t).
+Notation mem := Semantics.mem.
+
+Definition has_field (f : ident) (sv : Sval) : bool :=
+  match sv with
+  | ValBaseStruct fields =>
+      is_some (AList.get fields f)
+  | ValBaseHeader fields (Some true) =>
+      is_some (AList.get fields f)
+  | _ => false
+  end.
+
+Definition get (f : ident) (sv : Sval) : Sval :=
+  match sv with
+  | ValBaseStruct fields =>
+      force ValBaseNull (AList.get fields f)
+  | ValBaseHeader fields _ =>
+      force ValBaseNull (AList.get fields f)
+  | _ => ValBaseNull
+  end.
+
+Definition update (f : ident) (f_sv : Sval) (sv : Sval) : Sval :=
+  match sv with
+  | ValBaseStruct fields =>
+      ValBaseStruct (force fields (AList.set fields f f_sv))
+  | ValBaseHeader fields (Some true) =>
+      ValBaseHeader (force fields (AList.set fields f f_sv)) (Some true)
+  | _ => sv
+  end.
+
+Lemma get_some_get_set : forall {A} (l : AList.StringAList A) k (l' : AList.StringAList A) v1 v2,
+  AList.get l k = Some v1 ->
+  AList.get (force l' (AList.set l k v2)) k = Some v2.
+Proof.
+  intros.
+  erewrite AList.get_some_set by eauto.
+  apply AList.set_some_get.
+Qed.
+
+Lemma get_update : forall sv f f_sv,
+  has_field f sv ->
+  get f (update f f_sv sv) = f_sv.
+Proof.
+  intros.
+  destruct sv; try solve [inv H].
+  - unfold get, update, has_field in *.
+    destruct (AList.get fields f) eqn:?.
+    + erewrite get_some_get_set by eauto.
+      auto.
+    + inv H.
+  - destruct is_valid as [[] | ].
+    * unfold get, update, has_field in *.
+      destruct (AList.get fields f) eqn:?.
+      + erewrite get_some_get_set by eauto.
+        auto.
+      + inv H.
+    * inv H.
+    * inv H.
+Qed.
+
+End Members.
