core/SvalRefine.v
@@ -1,0 +1,193 @@
+Require Import Coq.NArith.BinNat.
+Require Import Poulet4.Typed.
+Require Import Poulet4.Syntax.
+Require Import Poulet4.Value.
+Require Import Poulet4.Semantics.
+Require Import ProD3.core.Coqlib.
+Require Import ProD3.core.Members.
+Require Import Poulet4.SyntaxUtil.
+Require Import Hammer.Plugin.Hammer.
+
+Section SvalRefine.
+
+Context {tags_t: Type} {tags_t_inhabitant : Inhabitant tags_t}.
+Notation Val := (@ValueBase bool).
+Notation Sval := (@ValueBase (option bool)).
+Notation Lval := (@ValueLvalue tags_t).
+
+Notation ident := (String.string).
+Notation path := (list ident).
+
+(* bit_refine a b means a includes b. *)
+Inductive bit_refine : option bool -> option bool -> Prop :=
+  | read_none : forall ob, bit_refine None ob
+  | read_some : forall b, bit_refine (Some b) (Some b).
+
+(* sval_refine a b means a includes b. *)
+Definition sval_refine := exec_val bit_refine.
+
+Definition rel_trans {A B C} (f : A -> B -> Prop) (g : B -> C -> Prop) (h : A -> C -> Prop) :=
+  forall a b c,
+    f a b ->
+    g b c ->
+    h a c.
+
+Section exec_val_trans.
+  Context {A B C : Type} (f : A -> B -> Prop) (g : B -> C -> Prop) (h : A -> C -> Prop).
+  Hypothesis H_rel_trans : rel_trans f g h.
+
+  Lemma Forall2_trans : forall v1 v2 v3,
+    Forall2 f v1 v2 ->
+    Forall2 g v2 v3 ->
+    Forall2 h v1 v3.
+  Proof.
+    intros v1 v2; revert v1.
+    induction v2; intros.
+    - inv H; inv H0; constructor.
+    - inv H; inv H0; constructor; eauto.
+  Qed.
+
+  Hint Resolve Forall2_trans : core.
+
+  Lemma exec_val_trans_case1 : forall vs1 vs2 vs3,
+    Forall
+      (fun v2 : ValueBase =>
+        forall v1 v3 : ValueBase, exec_val f v1 v2 -> exec_val g v2 v3 -> exec_val h v1 v3) vs2 ->
+    Forall2 (exec_val f) vs1 vs2 ->
+    Forall2 (exec_val g) vs2 vs3 ->
+    Forall2 (exec_val h) vs1 vs3.
+  Proof.
+    intros vs1 vs2; revert vs1.
+    induction vs2; intros; inv H1; inv H0; inv H; constructor; only 1 : apply H2; auto.
+  Qed.
+
+  Lemma exec_val_trans_case2 : forall (vs1 : list (ident * ValueBase)) vs2 vs3,
+    Forall
+      (fun '(_, v2) =>
+        forall v1 v3 : ValueBase, exec_val f v1 v2 -> exec_val g v2 v3 -> exec_val h v1 v3) vs2 ->
+    AList.all_values (exec_val f) vs1 vs2 ->
+    AList.all_values (exec_val g) vs2 vs3 ->
+    AList.all_values (exec_val h) vs1 vs3.
+  Proof.
+    intros vs1 vs2; revert vs1.
+    induction vs2; intros; inv H1; inv H0; inv H; constructor.
+    - destruct H4; destruct H5; split.
+      + congruence.
+      + destruct a; apply H2; auto.
+    - apply IHvs2; auto.
+  Qed.
+
+  (* rel_trans (exec_val f) (exec_val g) (exec_val h) *)
+  Lemma exec_val_trans : forall v1 v2 v3,
+    exec_val f v1 v2 ->
+    exec_val g v2 v3 ->
+    exec_val h v1 v3.
+  Proof.
+    intros v1 v2; revert v1.
+    induction v2 using custom_ValueBase_ind; intros * H_f H_g;
+      inv H_f; inv H_g;
+      constructor; eauto.
+    - eapply exec_val_trans_case1; eauto.
+    - eapply exec_val_trans_case2; eauto.
+    - eapply exec_val_trans_case2; eauto.
+    - eapply exec_val_trans_case2; eauto.
+    - eapply exec_val_trans_case2; eauto.
+    - eapply exec_val_trans_case1; eauto.
+  Qed.
+End exec_val_trans.
+
+Lemma bit_refine_trans : forall b1 b2 b3 : option bool,
+  bit_refine b1 b2 ->
+  bit_refine b2 b3 ->
+  bit_refine b1 b3.
+Proof.
+  intros.
+  inv H; inv H0; constructor.
+Qed.
+
+Lemma sval_refine_trans : forall sv1 sv2 sv3,
+  sval_refine sv1 sv2 ->
+  sval_refine sv2 sv3 ->
+  sval_refine sv1 sv3.
+Proof.
+  apply exec_val_trans. exact bit_refine_trans.
+Qed.
+
+Lemma all_values_get_some_rel : forall {A} (kvl kvl' : AList.StringAList A) f rel v v',
+  AList.all_values rel kvl kvl' ->
+  AList.get kvl f = Some v ->
+  AList.get kvl' f = Some v' ->
+  rel v v'.
+Proof.
+  intros.
+  induction H.
+  - inv H0.
+  - destruct x as [kx vx]; destruct y as [ky vy].
+    destruct H. simpl in H. subst ky.
+    destruct (String.string_dec f kx) eqn:?.
+    + rewrite AList.get_eq_cons in H1, H0 by auto.
+      inv H1; inv H0.
+      auto.
+    + rewrite AList.get_neq_cons in H1, H0 by auto.
+      auto.
+Qed.
+
+Lemma all_values_get_some_is_some : forall {A} (kvl kvl' : AList.StringAList A) f rel v,
+  AList.all_values rel kvl kvl' ->
+  AList.get kvl f = Some v ->
+  is_some (AList.get kvl' f).
+Proof.
+  intros.
+  induction H.
+  - inv H0.
+  - destruct x as [kx vx]; destruct y as [ky vy].
+    destruct H. simpl in H. subst ky.
+    destruct (String.string_dec f kx) eqn:?.
+    + rewrite AList.get_eq_cons in H0 |- * by auto.
+      auto.
+    + rewrite AList.get_neq_cons in H0 |- * by auto.
+      auto.
+Qed.
+
+Lemma all_values_get_some_is_some' : forall {A} (kvl kvl' : AList.StringAList A) f rel v,
+  AList.all_values rel kvl kvl' ->
+  AList.get kvl' f = Some v ->
+  is_some (AList.get kvl f).
+Proof.
+  intros.
+  induction H.
+  - inv H0.
+  - destruct x as [kx vx]; destruct y as [ky vy].
+    destruct H. simpl in H. subst ky.
+    destruct (String.string_dec f kx) eqn:?.
+    + rewrite AList.get_eq_cons in H0 |- * by auto.
+      auto.
+    + rewrite AList.get_neq_cons in H0 |- * by auto.
+      auto.
+Qed.
+
+Lemma sval_refine_get : forall sv sv' f,
+  sval_refine sv sv' ->
+  sval_refine (get f sv) (get f sv').
+Proof.
+  intros.
+  inv H; try solve [constructor].
+  - unfold get.
+    destruct (AList.get kvs f) eqn:H_get1; destruct (AList.get kvs' f) eqn:H_get2.
+    + eapply all_values_get_some_rel; eauto.
+    + epose proof (all_values_get_some_is_some _ _ _ _ _ ltac:(eauto) ltac:(eauto)) as H.
+      rewrite H_get2 in H. inv H.
+    + epose proof (all_values_get_some_is_some' _ _ _ _ _ ltac:(eauto) ltac:(eauto)) as H.
+      rewrite H_get1 in H. inv H.
+    + constructor.
+  - unfold get.
+    destruct (AList.get kvs f) eqn:H_get1; destruct (AList.get kvs' f) eqn:H_get2.
+    + eapply all_values_get_some_rel; eauto.
+    + epose proof (all_values_get_some_is_some _ _ _ _ _ ltac:(eauto) ltac:(eauto)) as H.
+      rewrite H_get2 in H. inv H.
+    + epose proof (all_values_get_some_is_some' _ _ _ _ _ ltac:(eauto) ltac:(eauto)) as H.
+      rewrite H_get1 in H. inv H.
+    + constructor.
+Qed.
+
+End SvalRefine.
